Challenge/Modexp/Submission/Proofs/Bytecode/UnrollPCs.lean
@@ -27,31 +27,31 @@ open YulEvmCompiler
   rw [Challenge.Modexp.Submission.Proofs.Bytecode.PCFast.instructionPC_eq_byteLength]
   rfl
 
-@[simp] theorem pc2414 : Artifact.submissionArtifact.instructionPC 1588 = 2115 := by
+@[simp] theorem pc2414 : Artifact.submissionArtifact.instructionPC 1970 = 2351 := by
   rw [Challenge.Modexp.Submission.Proofs.Bytecode.PCFast.instructionPC_eq_byteLength]
   rfl
 
-@[simp] theorem pc2415 : Artifact.submissionArtifact.instructionPC 1589 = 2116 := by
+@[simp] theorem pc2415 : Artifact.submissionArtifact.instructionPC 1971 = 2352 := by
   rw [Challenge.Modexp.Submission.Proofs.Bytecode.PCFast.instructionPC_eq_byteLength]
   rfl
 
-@[simp] theorem pc2416 : Artifact.submissionArtifact.instructionPC 1590 = 2118 := by
+@[simp] theorem pc2416 : Artifact.submissionArtifact.instructionPC 1972 = 2354 := by
   rw [Challenge.Modexp.Submission.Proofs.Bytecode.PCFast.instructionPC_eq_byteLength]
   rfl
 
-@[simp] theorem pc2417 : Artifact.submissionArtifact.instructionPC 1591 = 2119 := by
+@[simp] theorem pc2417 : Artifact.submissionArtifact.instructionPC 1973 = 2355 := by
   rw [Challenge.Modexp.Submission.Proofs.Bytecode.PCFast.instructionPC_eq_byteLength]
   rfl
 
-@[simp] theorem pc2554 : Artifact.submissionArtifact.instructionPC 1620 = 2156 := by
+@[simp] theorem pc2554 : Artifact.submissionArtifact.instructionPC 2002 = 2392 := by
   rw [Challenge.Modexp.Submission.Proofs.Bytecode.PCFast.instructionPC_eq_byteLength]
   rfl
 
-@[simp] theorem pc2555 : Artifact.submissionArtifact.instructionPC 1621 = 2157 := by
+@[simp] theorem pc2555 : Artifact.submissionArtifact.instructionPC 2003 = 2393 := by
   rw [Challenge.Modexp.Submission.Proofs.Bytecode.PCFast.instructionPC_eq_byteLength]
   rfl
 
-@[simp] theorem pc2556 : Artifact.submissionArtifact.instructionPC 1622 = 2159 := by
+@[simp] theorem pc2556 : Artifact.submissionArtifact.instructionPC 2004 = 2395 := by
   rw [Challenge.Modexp.Submission.Proofs.Bytecode.PCFast.instructionPC_eq_byteLength]
   rfl
 
